Trying to prove [msiSv_impl_InvTrs]

src/Ex/MsiSvSim.v
@@ -11,6 +11,26 @@ Open Scope list.
 Open Scope hvec.
 Open Scope fmap.
 
+Notation "A <-- OA ; CONT" :=
+  (OA >>=[False] (fun A => CONT)) (at level 15, right associativity).
+Notation "A <+- OA ; CONT" :=
+  (OA >>=[True] (fun A => CONT)) (at level 15, right associativity).
+
+Fixpoint caseDec {A B} (dec: forall a1 a2: A, {a1 = a2} + {a1 <> a2})
+         (a: A) (def: B) (cs: list (A * B)) :=
+  match cs with
+  | nil => def
+  | (ca, cp) :: cs' =>
+    if dec a ca then cp else caseDec dec a def cs'
+  end.
+
+Notation "x : t" := (x, t) (at level 90, only parsing): cases_scope.
+Notation "| xt1 | xt2 | .. | xtn" :=
+  (cons xt1 (cons xt2 .. (cons xtn nil) ..)) (at level 95, only parsing): cases_scope.
+Delimit Scope cases_scope with cases.
+Notation "'match' 'case' X 'on' DEC 'default' DEF 'with' CS 'end'" :=
+  (caseDec DEC X DEF CS%cases) (only parsing).
+
 Definition Mii := (IdxT * IdxT)%type.
 
 Definition mii_dec: forall mii1 mii2: Mii, {mii1 = mii2} + {mii1 <> mii2}.
@@ -27,16 +47,29 @@ Definition miisOf (msgs: list (Id Msg)): list Mii :=
   map miiOf msgs.
 
 Definition AtomicMsgOutsInv {oifc} (mp: MsgOutPred oifc)
-           (abf: list Mii -> list Mii):
-  list (Id Msg) -> list (Id Msg) -> MState oifc -> MState oifc -> Prop :=
-  fun inits eouts pst nst =>
-    SubList (miisOf eouts) (abf (miisOf inits)) /\
-    Forall (fun eout => mp eout nst.(bst_oss)) eouts.
+           (abf: list Mii -> list Mii)
+           (inits eouts: list (Id Msg)) (nst: MState oifc): Prop :=
+  SubList (miisOf eouts) (abf (miisOf inits)) /\
+  Forall (fun eout => mp eout nst.(bst_oss)) eouts.
 
-Ltac disc_AtomicMsgOutsInv :=
-  match goal with
-  | [H: AtomicMsgOutsInv _ _ _ _ _ _ |- _] => destruct H
-  end.
+Definition AtomicLocksInv {oifc}
+           (lp: list Mii -> IdxT -> ORq Msg -> Prop)
+           (inits: list (Id Msg)) (hst: MHistory) (nst: MState oifc): Prop :=
+  forall oidx,
+    In oidx (oindsOf hst) ->
+    orq <-- (bst_orqs nst)@[oidx]; lp (miisOf inits) oidx orq.
+
+Definition AtomicInv {oifc}
+           (mp: MsgOutPred oifc) (abf: list Mii -> list Mii)
+           (lp: list Mii -> IdxT -> ORq Msg -> Prop):
+  list (Id Msg) (* inits *) ->
+  MState oifc (* starting state *) ->
+  MHistory (* atomic history *) ->
+  list (Id Msg) (* eouts *) ->
+  MState oifc (* ending state *) -> Prop :=
+  fun inits st1 hst eouts st2 =>
+    AtomicMsgOutsInv mp abf inits eouts st2 /\
+    AtomicLocksInv lp inits hst st2.
 
 Section Inv.
 
@@ -142,50 +175,47 @@ Section Inv.
       apply DisjList_comm, sys_minds_sys_merss_DisjList.
     Qed.
 
-    Notation "A <-- OA ; CONT" :=
-      (OA >>=[False] (fun A => CONT)) (at level 15, right associativity).
-
-    Fixpoint caseDec {A B} (dec: forall a1 a2: A, {a1 = a2} + {a1 <> a2})
-             (a: A) (def: B) (cs: list (A * B)) :=
-      match cs with
-      | nil => def
-      | (ca, cp) :: cs' =>
-        if dec a ca then cp else caseDec dec a def cs'
-      end.
-
-    Notation "x : t" := (x, t) (at level 90, only parsing): cases_scope.
-    Notation "| xt1 | xt2 | .. | xtn" :=
-      (cons xt1 (cons xt2 .. (cons xtn nil) ..)) (at level 95, only parsing): cases_scope.
-    Delimit Scope cases_scope with cases.
-    Notation "'match' 'case' X 'on' DEC 'default' DEF 'with' CS 'end'" :=
-      (caseDec DEC X DEF CS%cases) (only parsing).
-
     Definition MsiSvMsgOutPred: MsgOutPred ImplOStateIfc :=
       fun eout oss =>
-        post <-- oss@[parentIdx];
-          cost1 <-- oss@[child1Idx];
-          cost2 <-- oss@[child2Idx];
-          match case (miiOf eout)
-                     on mii_dec
-                     default True
-          with
-          | (pc1, msiRsS): 
-              post#[implStatusIdx] = msiS /\ cost2#[implStatusIdx] = msiS
-          | (pc2, msiRsS):
-              post#[implStatusIdx] = msiS /\ cost1#[implStatusIdx] = msiS
-          | (pc1, msiRsM): 
-              post#[implStatusIdx] = msiM /\ cost2#[implStatusIdx] = msiI
-          | (pc2, msiRsM):
-              post#[implStatusIdx] = msiM /\ cost1#[implStatusIdx] = msiI
-          | (c1pRs, msiDownRsS): cost1#[implStatusIdx] = msiS
-          | (c2pRs, msiDownRsS): cost2#[implStatusIdx] = msiS
-          | (c1pRs, msiDownRsM): cost1#[implStatusIdx] = msiI
-          | (c2pRs, msiDownRsM): cost2#[implStatusIdx] = msiI
-          end.
+        match case (miiOf eout) on mii_dec default True with
+        | (pc1, msiRsS): 
+            post <-- oss@[parentIdx];
+            cost2 <-- oss@[child2Idx];
+            (post#[implStatusIdx] = msiS /\ cost2#[implStatusIdx] = msiS)
+        | (pc2, msiRsS):
+            post <-- oss@[parentIdx];
+            cost1 <-- oss@[child1Idx];
+            (post#[implStatusIdx] = msiS /\ cost1#[implStatusIdx] = msiS)
+        | (pc1, msiRsM): 
+            post <-- oss@[parentIdx];
+            cost2 <-- oss@[child2Idx];
+            (post#[implStatusIdx] = msiM /\ cost2#[implStatusIdx] = msiI)
+        | (pc2, msiRsM):
+            post <-- oss@[parentIdx];
+            cost1 <-- oss@[child1Idx];
+            (post#[implStatusIdx] = msiM /\ cost1#[implStatusIdx] = msiI)
+        | (c1pRs, msiDownRsS):
+            cost1 <-- oss@[child1Idx];
+            (cost1#[implStatusIdx] = msiS)
+        | (c2pRs, msiDownRsS):
+            cost2 <-- oss@[child2Idx];
+            (cost2#[implStatusIdx] = msiS)
+        | (c1pRs, msiDownRsM):
+            cost1 <-- oss@[child1Idx];
+            (cost1#[implStatusIdx] = msiI)
+        | (c2pRs, msiDownRsM):
+            cost2 <-- oss@[child2Idx];
+            (cost2#[implStatusIdx] = msiI)
+        end.
 
     Lemma msiSvMsgOutPred_good:
       GoodMsgOutPred topo MsiSvMsgOutPred.
     Proof.
+      red; intros.
+      repeat split.
+      - red; intros.
+        red in H; dest.
+        (** TODO: need a lemma [rsEdgeUpFrom dtr oidx = Some _ -> In oidx (indsOf dtr)] *)
     Admitted.
 
     Definition msiSvAtomicBoundF (inits: list Mii): list Mii :=
@@ -208,9 +238,67 @@ Section Inv.
           [(ce2, Spec.evictRs); (c2pRq, msiRqI); (pc2, msiRsI)]
       end.
 
-    Ltac disc_rule_custom ::=
-      try disc_AtomicMsgOutsInv.
+    Definition MsiSvLockPred (inits: list Mii) (oidx: IdxT) (orq: ORq Msg): Prop :=
+      match case inits on miis_dec default False with
+      | [(ec1, Spec.getRq)]:
+          match case oidx on eq_nat_dec default True with
+          | child1Idx:
+              rqiu <+- orq@[upRq];
+              (rqiu.(rqi_minds_rss) = [pc1])
+          | parentIdx:
+              rqid <+- orq@[downRq];
+              (rqid.(rqi_minds_rss) = [c2pRs])
+          end
+      | [(ec1, Spec.setRq)]:
+          match case oidx on eq_nat_dec default True with
+          | child1Idx:
+              rqiu <+- orq@[upRq];
+              (rqiu.(rqi_minds_rss) = [pc1])
+          | parentIdx:
+              rqid <+- orq@[downRq];
+              (rqid.(rqi_minds_rss) = [c2pRs])
+          end
+      | [(ec1, Spec.evictRq)]:
+          match case oidx on eq_nat_dec default True with
+          | child1Idx:
+              rqiu <+- orq@[upRq];
+              (rqiu.(rqi_minds_rss) = [pc1])
+          | parentIdx: True
+          end
+      | [(ec2, Spec.getRq)]:
+          match case oidx on eq_nat_dec default True with
+          | child2Idx:
+              rqiu <+- orq@[upRq];
+              (rqiu.(rqi_minds_rss) = [pc2])
+          | parentIdx:
+              rqid <+- orq@[downRq];
+              (rqid.(rqi_minds_rss) = [c1pRs])
+          end
+      | [(ec2, Spec.setRq)]:
+          match case oidx on eq_nat_dec default True with
+          | child2Idx:
+              rqiu <+- orq@[upRq];
+              (rqiu.(rqi_minds_rss) = [pc2])
+          | parentIdx:
+              rqid <+- orq@[downRq];
+              (rqid.(rqi_minds_rss) = [c1pRs])
+          end
+      | [(ec2, Spec.evictRq)]:
+          match case oidx on eq_nat_dec default True with
+          | child2Idx:
+              rqiu <+- orq@[upRq];
+              (rqiu.(rqi_minds_rss) = [pc2])
+          | parentIdx: True
+          end
+      end.
 
+    Ltac disc_rule_custom ::=
+      repeat
+        match goal with
+        | [H: AtomicInv _ _ _ _ _ _ _ _ |- _] => red in H; dest
+        | [H: AtomicMsgOutsInv _ _ _ _ _ |- _] => red in H; dest
+        end.
+    
     Ltac atomic_non_init_bound_exfalso_step :=
       match goal with
       | [H1: SubList [_] ?eouts, H2: SubList (miisOf ?eouts) _ |- _] =>
@@ -219,37 +307,130 @@ Section Inv.
         clear -Hs; apply SubList_singleton_In in Hs; cbn in Hs
       | [H: context[miis_dec ?miis1 ?miis2] |- _] =>
         destruct (miis_dec miis1 miis2) in H;
-        try (dest_in; discriminate)
+        try (Common.dest_in; discriminate)
       end.
 
-    Ltac atomic_non_init_bound_exfalso :=
-      exfalso;
-      disc_rule_conds; solve_rule_conds_const;
-      repeat atomic_non_init_bound_exfalso_step.
-    
     Lemma msiSv_impl_InvTrs: InvTrs impl ImplStateMSI.
     Proof.
       eapply inv_atomic_InvTrs;
         [red; intros; eapply msiSv_impl_InvTrs_ext_in; eauto
         |red; intros; eapply msiSv_impl_InvTrs_ext_out; eauto
         |].
-      instantiate (1:= AtomicMsgOutsInv MsiSvMsgOutPred msiSvAtomicBoundF).
+      instantiate (1:= AtomicInv
+                         MsiSvMsgOutPred
+                         msiSvAtomicBoundF
+                         MsiSvLockPred).
 
+      (** TODO: make an ltac for below *)
       red; intros.
       destruct H1.
-
       generalize dependent ist2.
       induction H3; simpl; intros; subst.
-      - admit.
+      
+      - inv_steps; inv_step.
+        dest_in.
+
+        1: {
+          disc_rule_conds_ex.
+          simpl; split; [split|].
+          * (* [AtomicMsgOutsInv] *)
+            split.
+            { simpl; unfold miiOf; simpl.
+              rewrite H8; cbn.
+              apply SubList_cons; [|apply SubList_nil].
+              simpl; tauto.
+            }
+            { simpl; repeat constructor. }
+          * (* [AtomicLocksInv] *)
+            red; intros; dest_in.
+            repeat (simpl; mred).
+            unfold miiOf; simpl.
+            rewrite H8; cbn.
+            unfold upRq; rewrite H5.
+            simpl; auto.
+          * (* [ImplStateMSI] *)
+            replace (oss +[child1Idx <- pos]) with oss by meq.
+            destruct H0 as [cv ?].
+            red in H0; simpl in H0; dest.
+            exists cv.
+            red; simpl; split; [assumption|].
+
+            do 2 red; intros.
+            red; intros.
+            rewrite findQ_not_In_enqMP
+              by (intro Hx; subst; dest_in; discriminate).
+            rewrite findQ_not_In_deqMP
+              by (intro Hx; subst; dest_in; discriminate).
+            apply H2; auto.
+        }
+
+        1: {
+          disc_rule_conds_ex.
+          simpl; split; [split|].
+          * (* [AtomicMsgOutsInv] *)
+            split.
+            { simpl; unfold miiOf; simpl.
+              rewrite H7; cbn.
+              apply SubList_cons; [|apply SubList_nil].
+              simpl; tauto.
+            }
+            { simpl; repeat constructor. }
+          * (* [AtomicLocksInv] *)
+            red; intros; dest_in.
+            repeat (simpl; mred).
+            unfold miiOf; simpl.
+            rewrite H7.
+            red; simpl.
+            mred.
+          * (* [ImplStateMSI] *)
+            replace (oss +[child1Idx <- pos]) with oss by meq.
+            destruct H0 as [cv ?].
+            red in H0; simpl in H0; dest.
+            exists cv.
+            red; simpl; split; [assumption|].
+
+            do 2 red; intros.
+            red; intros.
+
+            destruct (eq_nat_dec midx c1pRq).
+            { subst.
+              rewrite findQ_In_enqMP.
+              apply Forall_app.
+              { rewrite findQ_not_In_deqMP
+                  by (intro Hx; subst; dest_in; discriminate).
+                apply H2; auto.
+              }
+              { repeat constructor.
+                red; intros.
+                clear H3; dest_in; discriminate.
+              }
+            }
+            { rewrite findQ_not_In_enqMP by assumption.
+              rewrite findQ_not_In_deqMP
+                by (intro Hx; subst; dest_in; discriminate).
+              apply H2; auto.
+            }
+        }
+
+        2: {
+          exfalso.
+          disc_rule_conds_ex.
+          apply SubList_singleton_In in H1; dest_in; discriminate.
+        }
+
+        all: admit.
 
       - inv_steps.
         specialize (IHAtomic H1 _ H9); dest.
         (** For each rule, *)
         inv_step; dest_in.
 
-        + atomic_non_init_bound_exfalso.
-        + atomic_non_init_bound_exfalso.
-        + 
+        1: {
+          exfalso.
+          disc_rule_conds_ex.
+          repeat atomic_non_init_bound_exfalso_step.
+        }
+        
     Admitted.
 
     Lemma ImplStateMSI_init:
